feat: automata decision procedure (#790)
Co-authored-by: Léo Stefanesco <leo.lveb@gmail.com>

SSA/Experimental/Bits/AutoStructs/Defs.lean
@@ -3,10 +3,28 @@ Released under Apache 2.0 license as described in the file LICENSE.
 -/
 import Mathlib.Data.Bool.Basic
 import Mathlib.Data.Fin.Basic
+import Mathlib.Tactic
 import SSA.Projects.InstCombine.ForLean
 import SSA.Experimental.Bits.Fast.BitStream
+import SSA.Experimental.Bits.AutoStructs.ForMathlib
 
 namespace AutoStructs
+
+-- A bunch of maps from `Fin n` to `Fin m` that we use to
+-- lift and project variables when we interpret formulas
+def liftMaxSucc1 (n m : Nat) : Fin (n + 1) → Fin (max n m + 2) :=
+  fun k => if _ : k = n then Fin.last (max n m) else k.castLE (by omega)
+def liftMaxSucc2 (n m : Nat) : Fin (m + 1) → Fin (max n m + 2) :=
+  fun k => if _ : k = m then Fin.last (max n m + 1) else k.castLE (by omega)
+def liftLast2 n : Fin 2 → Fin (n + 2)
+| 0 => n
+| 1 => Fin.last (n + 1)
+def liftExcept2 n : Fin n → Fin (n + 2) :=
+  fun k => Fin.castLE (by omega) k
+def liftMax1 (n m : Nat) : Fin n → Fin (max n m) :=
+  fun k => k.castLE (by omega)
+def liftMax2 (n m : Nat) : Fin m → Fin (max n m) :=
+  fun k => k.castLE (by omega)
 
 /-!
 # Term Language
@@ -39,10 +57,6 @@ inductive Term : Type
 | sub : Term → Term → Term
 /-- Negation -/
 | neg : Term → Term
-/-- Increment (i.e., add one) -/
-| incr : Term → Term
-/-- Decrement (i.e., subtract one) -/
-| decr : Term → Term
 deriving Repr
 -- /-- `repeatBit` is an operation that will repeat the infinitely repeat the
 -- least significant `true` bit of the input.
@@ -81,8 +95,6 @@ a term like `var 10` only has a single free variable, but its arity will be `11`
 | add t₁ t₂ => max (arity t₁) (arity t₂)
 | sub t₁ t₂ => max (arity t₁) (arity t₂)
 | neg t => arity t
-| incr t => arity t
-| decr t => arity t
 -- | repeatBit t => arity t
 
 
@@ -122,13 +134,19 @@ and only require that many bitstream values to be given in `vars`.
       let x₂ := t₂.evalFin (fun i => vars (Fin.castLE (by simp [arity]) i))
       x₁ - x₂
   | neg t       => -(Term.evalFin t vars)
-  | incr t      => Term.evalFin t vars + 1
-  | decr t      => Term.evalFin t vars - 1
   -- | repeatBit t => BitStream.repeatBit (Term.evalFin t vars)
+
+lemma evalFin_eq {t : Term} {vars1 : Fin t.arity → BitVec w1} {vars2 : Fin t.arity → BitVec w2} :
+    ∀ (heq : w1 = w2),
+    (∀ n, vars1 n = heq ▸ vars2 n) →
+    t.evalFin vars1 = heq ▸ t.evalFin vars2 := by
+  rintro rfl heqs
+  simp only
+  congr; ext1; simp_all
 
 @[simp] def Term.evalNat (t : Term) (vars : Nat → BitVec w) : BitVec w :=
   match t with
-  | var n => vars (Fin.last n)
+  | var n => vars n
   | zero    => BitVec.zero w
   | one     => 1
   | negOne  => -1
@@ -155,8 +173,6 @@ and only require that many bitstream values to be given in `vars`.
       let x₂ := t₂.evalNat vars
       x₁ - x₂
   | neg t       => -(Term.evalNat t vars)
-  | incr t      => Term.evalNat t vars + 1
-  | decr t      => Term.evalNat t vars - 1
   -- | repeatBit t => BitStream.repeatBit (Term.evalFin t vars)
 @[simp] def Term.evalFinStream (t : Term) (vars : Fin (arity t) → BitStream) : BitStream :=
   match t with
@@ -186,8 +202,9 @@ and only require that many bitstream values to be given in `vars`.
       let x₂ := t₂.evalFinStream (fun i => vars (Fin.castLE (by simp [arity]) i))
       x₁ - x₂
   | neg t       => -(Term.evalFinStream t vars)
-  | incr t      => BitStream.incr (Term.evalFinStream t vars)
-  | decr t      => BitStream.decr (Term.evalFinStream t vars)
+
+def Term.language (t : Term) : Set (BitVecs (t.arity + 1)) :=
+  { bvs : BitVecs (t.arity + 1) | t.evalFin (fun n => bvs.bvs.get n) = bvs.bvs.get t.arity }
 
 inductive RelationOrdering
 | lt | le | gt | ge
@@ -199,8 +216,7 @@ inductive Relation
 | unsigned (ord : RelationOrdering)
 deriving Repr
 
-@[simp]
-def evalRelation {w} (rel : Relation) (bv1 bv2 : BitVec w) : Bool :=
+def evalRelation (rel : Relation) {w} (bv1 bv2 : BitVec w) : Bool :=
   match rel with
   | .eq => bv1 = bv2
   | .signed .lt => bv1 <ₛ bv2
@@ -212,11 +228,19 @@ def evalRelation {w} (rel : Relation) (bv1 bv2 : BitVec w) : Bool :=
   | .unsigned .gt => bv1 >ᵤ bv2
   | .unsigned .ge => bv1 ≥ᵤ bv2
 
+@[simp]
+lemma evalRelation_coe (rel : Relation) (bv1 bv2 : BitVec w1) (heq : w1 = w2) :
+    evalRelation rel (heq ▸ bv1) (heq ▸ bv2) = evalRelation rel bv1 bv2 := by
+  rcases heq; simp
+
+@[simp]
+def Relation.language (rel : Relation) : Set (BitVecs 2) :=
+  { bvs | evalRelation rel (bvs.bvs.get 0) (bvs.bvs.get 1) }
+
 inductive Binop
 | and | or | impl | equiv
 deriving Repr
 
-@[simp]
 def evalBinop (op : Binop) (b1 b2 : Bool) : Bool :=
   match op with
   | .and => b1 && b2
@@ -231,6 +255,14 @@ def evalBinop' (op : Binop) (b1 b2 : Prop) : Prop :=
   | .or => b1 ∨ b2
   | .impl => b1 → b2
   | .equiv => b1 ↔ b2
+
+def langBinop (op : Binop) (l1 l2 : Set (BitVecs n)) : Set (BitVecs n) :=
+  match op with
+  | .and => l1 ∩ l2
+  | .or => l1 ∪ l2
+  | .impl => l1ᶜ ∪ l2
+  | .equiv => (l1ᶜ ∪ l2) ∩ (l2ᶜ ∪ l1)
+
 inductive Unop
 | neg
 deriving Repr
@@ -266,6 +298,206 @@ def Formula.sat {w : Nat} (φ : Formula) (ρ : Fin φ.arity → BitVec w) : Bool
   | .msbSet t => (t.evalFin ρ).msb
 
 @[simp]
+def _root_.Set.lift (f : Fin n → Fin m) (bvs : Set (BitVecs n)) : Set (BitVecs m) :=
+  BitVecs.transport f ⁻¹' bvs
+
+@[simp]
+def _root_.Set.proj (f : Fin n → Fin m) (bvs : Set (BitVecs m)) : Set (BitVecs n) :=
+  BitVecs.transport f '' bvs
+
+@[simp]
+def langMsb : Set (BitVecs 1) := { bvs | bvs.bvs.get 0 |>.msb }
+
+@[simp]
+def Formula.language (φ : Formula) : Set (BitVecs φ.arity) :=
+  match φ with
+  | .atom rel t1 t2 =>
+    let l1 := t1.language.lift (liftMaxSucc1 (FinEnum.card $ Fin t1.arity) (FinEnum.card $ Fin t2.arity))
+    let l2 := t2.language.lift (liftMaxSucc2 (FinEnum.card $ Fin t1.arity) (FinEnum.card $ Fin t2.arity))
+    let lrel := rel.language.lift $ liftLast2 (max (FinEnum.card (Fin t1.arity)) (FinEnum.card (Fin t2.arity)))
+    let l := lrel ∩ l1 ∩ l2
+    l.proj (liftExcept2 _)
+  | .unop .neg φ => φ.languageᶜ
+  | .binop op φ1 φ2 =>
+    let l1 := φ1.language.lift $ liftMax1 φ1.arity φ2.arity
+    let l2 := φ2.language.lift $ liftMax2 φ1.arity φ2.arity
+    langBinop op l1 l2
+  | .msbSet t =>
+    let lmsb := langMsb.lift $ fun _ => Fin.last t.arity
+    let l' := t.language ∩ lmsb
+    l'.proj fun n => n.castLE (by simp [Formula.arity, FinEnum.card])
+
+lemma helper1 : (k = 0) → (x ::ᵥ vs).get k = x := by rintro rfl; simp
+lemma helper2 : (k = 1) → (x ::ᵥ y ::ᵥ vs).get k = y := by rintro rfl; simp [Mathlib.Vector.get]
+lemma msb_coe {x : BitVec w1} (heq : w1 = w2) : x.msb = (heq ▸ x).msb := by rcases heq; simp
+
+lemma formula_language_case_atom :
+    let φ := Formula.atom rel t1 t2
+    φ.language = λ (bvs : BitVecs φ.arity) => (φ.sat (fun k => bvs.bvs.get k) = true) := by
+  unfold Formula.language
+  rintro φ
+  let n := φ.arity
+  unfold φ
+  dsimp (config := { zeta := false })
+  lift_lets
+  intros l1 l2 lrel l
+  ext bvs
+  constructor
+  · intros h; simp at h
+    obtain ⟨bvsb, h, heqb⟩ := h
+    unfold l at h
+    simp at h
+    unfold lrel l1 l2 at h
+    obtain ⟨⟨hrel, h1⟩, h2⟩ := h
+    have _ : n+1 < bvsb.bvs.length := by simp_all [n]
+    have _ : n < bvsb.bvs.length := by simp_all [n]
+    have hrel : evalRelation rel (bvsb.bvs.get n) (bvsb.bvs.get (Fin.last (n + 1))) := by
+      simp at hrel
+      apply hrel
+    have ht1 : bvsb.bvs.get n = t1.evalFin fun n => bvsb.bvs.get n := by
+      unfold Term.language at h1
+      simp [Mathlib.Vector.transport, liftMaxSucc1] at h1
+      unfold n; simp; rw [←h1]
+      congr; ext1 k
+      split_ifs with h
+      · exfalso
+        have _ : k < t1.arity := by simp
+        have _ : k = t1.arity := by rcases k with ⟨k, hk⟩; simp_all [Fin.last]
+        omega
+      · congr; ext; simp; rw [Nat.mod_eq_of_lt]; omega
+    have ht2 : bvsb.bvs.get (Fin.last (n+1)) = t2.evalFin fun n => bvsb.bvs.get n := by
+      unfold Term.language at h2
+      simp [Mathlib.Vector.transport, liftMaxSucc2] at h2
+      unfold n; simp only [Formula.arity, Fin.natCast_self]; rw [←h2]
+      congr; ext1 k
+      split_ifs with h
+      · exfalso
+        have _ : k < t2.arity := by simp
+        have _ : k = t2.arity := by rcases k with ⟨k, hk⟩; simp_all [Fin.last]
+        omega
+      · congr; ext; simp; rw [Nat.mod_eq_of_lt]; omega
+    have hw : bvsb.w = bvs.w := by rw [←heqb]; simp
+    have heq1 : (t1.evalFin fun n => bvsb.bvs.get n) =
+        hw ▸ t1.evalFin fun n => bvs.bvs.get $ n.castLE (by simp) := by
+      apply evalFin_eq hw; intros k
+      rcases bvs with ⟨w, bvs⟩; rcases hw
+      injection heqb with _ heqb; rw [←heqb]
+      simp [Mathlib.Vector.transport, liftExcept2]
+      congr; ext; simp; omega
+    have heq2 : (t2.evalFin fun n => bvsb.bvs.get n) =
+        hw ▸ t2.evalFin fun n => bvs.bvs.get $ n.castLE (by simp) := by
+      apply evalFin_eq hw; intros k
+      rcases bvs with ⟨w, bvs⟩; rcases hw
+      injection heqb with _ heqb; rw [←heqb]
+      simp [Mathlib.Vector.transport, liftExcept2]
+      congr; ext; simp; omega
+    rw [ht1, ht2, heq1, heq2, evalRelation_coe] at hrel
+    dsimp only [Set.instMembership, Set.Mem]
+    simp_all
+  · intros h
+    simp
+    let bv1 := t1.evalFin fun k => bvs.bvs.get $ k.castLE (by simp)
+    let bv2 := t2.evalFin fun k => bvs.bvs.get $ k.castLE (by simp)
+    use ⟨bvs.w, bvs.bvs.append $ bv1 ::ᵥ bv2 ::ᵥ Mathlib.Vector.nil⟩
+    rcases bvs with ⟨w, bvs⟩
+    simp
+    constructor
+    · unfold l; simp; split_ands
+      · unfold lrel; simp only [Fin.isValue, BitVecs.transport_getElem,
+          liftLast2, Set.mem_setOf_eq, Fin.val_last, le_add_iff_nonneg_right, zero_le,
+          Mathlib.Vector.append_get_ge]
+        rw [Mathlib.Vector.append_get_ge (by dsimp; rw [Nat.mod_eq_of_lt]; omega)]
+        simp [Set.instMembership, Set.Mem] at h
+        convert h using 2
+        · apply helper1; ext; simp; rw [Nat.mod_eq_of_lt] <;> omega
+        · apply helper2; ext; simp
+      · unfold l1 Term.language; simp [Mathlib.Vector.transport, liftMaxSucc1]
+        rw [Mathlib.Vector.append_get_ge (by dsimp; rw [Nat.mod_eq_of_lt]; omega)]
+        rw [helper1 (by ext; simp; rw [Nat.mod_eq_of_lt] <;> omega)]
+        unfold bv1
+        congr; ext1 k; split_ifs
+        · exfalso
+          have _ : k < t1.arity := by simp
+          have _ : k = t1.arity := by rcases k with ⟨k, hk⟩; simp_all [Fin.last]
+          omega
+        · simp; congr 1
+      · unfold l2 Term.language; simp [Mathlib.Vector.transport, liftMaxSucc2]
+        rw [helper2 (by ext; simp)]
+        unfold bv2
+        congr; ext1 k; split_ifs
+        · exfalso
+          have _ : k < t2.arity := by simp
+          have _ : k = t2.arity := by rcases k with ⟨k, hk⟩; simp_all [Fin.last]
+          omega
+        · simp; congr 1
+    · ext1; simp
+      next i =>
+        simp [Mathlib.Vector.transport, liftExcept2]
+        rw [Mathlib.Vector.append_get_lt i.isLt]
+        congr 1
+
+theorem formula_language (φ : Formula) :
+    φ.language = { (bvs : BitVecs φ.arity) | φ.sat (fun k => bvs.bvs.get k) = true } := by
+  let n : Nat := φ.arity
+  induction φ
+  case atom rel t1 t2 =>
+    apply formula_language_case_atom
+  case unop op φ ih =>
+    rcases op; simp [ih, Set.compl_def]
+  case binop op φ1 φ2 ih1 ih2 =>
+    unfold Formula.language
+    ext1 bvs
+    simp [ih1, ih2]
+    have heq1 : (φ1.sat fun k => bvs.bvs.get (liftMax1 φ1.arity φ2.arity k)) = true ↔
+           (φ1.sat fun n => bvs.bvs.get (Fin.castLE (by simp) n)) = true := by
+      simp; congr
+    have heq2 : (φ2.sat fun k => bvs.bvs.get (liftMax2 φ1.arity φ2.arity k)) = true ↔
+           (φ2.sat fun n => bvs.bvs.get (Fin.castLE (by simp) n)) = true := by
+      simp; congr
+    rcases op <;>
+      simp [evalBinop, langBinop, Set.compl, Set.instMembership,
+        Set.Mem, Mathlib.Vector.transport] <;> aesop
+  case msbSet t =>
+    ext1 bvs; simp only [Formula.arity, Formula.language, Set.proj, Set.lift, langMsb, Fin.isValue,
+      Set.preimage_setOf_eq, Set.mem_image, Set.mem_inter_iff,
+      Set.mem_setOf_eq, Formula.sat]
+    rcases bvs with ⟨w, bvs⟩
+    constructor
+    · rintro ⟨bvsb, ⟨ht, hmsb⟩, heq⟩
+      simp only [Fin.isValue, Formula.arity] at ht hmsb ⊢
+      unfold Term.language at ht
+      simp only [BitVecs.transport, Mathlib.Vector.transport] at hmsb
+      simp at ht; rw [←ht] at hmsb; rw [←hmsb]
+      simp [BitVecs.transport] at heq
+      obtain ⟨hw, hbvs⟩ := heq
+      simp [hw]; congr 1; simp [hw]
+      rcases hw; simp
+      congr 1; ext1 k
+      simp at hbvs; simp [←hbvs, Mathlib.Vector.transport]; congr
+    · intros heq
+      use ⟨w,
+        bvs.append ((t.evalFin fun k => bvs.get $ k.castLE (by simp)) ::ᵥ Mathlib.Vector.nil)⟩
+      unfold Term.language
+      simp [BitVecs.transport, Mathlib.Vector.transport] at heq ⊢
+      constructor; assumption
+      ext1 k; simp; congr 1
+
+/--
+The formula `φ` is true for evey valuation.
+-/
+@[simp]
+def Formula.Tautology (φ : Formula) := φ.language = ⊤
+
+/--
+The formula `φ` is true for evey valuation made up of non-empty bitvectors.
+-/
+@[simp]
+def Formula.Tautology' (φ : Formula) := φ.language ∪ BitVecs0 = ⊤
+
+/--
+Same as `Formula.sat` but the environment is indexed by unbounded natural number.
+-/
+@[simp]
 def Formula.sat' {w : Nat} (φ : Formula) (ρ : Nat → BitVec w) : Prop :=
   match φ with
   | .atom rel t1 t2 =>
@@ -278,6 +510,29 @@ def Formula.sat' {w : Nat} (φ : Formula) (ρ : Nat → BitVec w) : Prop :=
     let b2 := φ2.sat' ρ
     evalBinop' op b1 b2
   | .msbSet t => (t.evalNat ρ).msb
+
+lemma evalFin_evalNat (t : Term):
+    t.evalFin (fun k => ρ k.val) = t.evalNat ρ := by
+  induction t <;> simp_all
+
+lemma sat_impl_sat' {φ : Formula} :
+    (φ.sat fun k => ρ k.val) ↔ φ.sat' ρ := by
+  induction φ
+  case atom rel t1 t2 =>
+    simp [←evalFin_evalNat]
+  case binop op φ1 φ2 ih1 ih2 =>
+    simp [evalBinop, ←ih1, ←ih2]
+    rcases op <;> simp
+    rw [←Bool.eq_false_eq_not_eq_true]
+    tauto
+  case unop op φ ih => rcases op; simp [←ih]
+  case msbSet t =>
+    simp [←evalFin_evalNat]
+
+lemma env_to_bvs (φ : Formula) (ρ : Fin φ.arity → BitVec w) :
+    let bvs : BitVecs φ.arity := ⟨w, Mathlib.Vector.ofFn fun k => ρ k⟩
+    ρ = fun k => bvs.bvs.get k := by
+  simp
 
 @[simp]
 abbrev envOfArray {w} (a : Array (BitVec w)) : Nat → BitVec w := fun n => a.getD n 0
