SSA/Experimental/Bits/AutoStructs/ForMathlib.lean
@@ -1,0 +1,639 @@
+import Batteries.Data.Fin.Basic
+import Mathlib.Computability.NFA
+import Mathlib.Data.FinEnum
+import Mathlib.Data.Vector.Basic
+import Mathlib.Data.Vector.Defs
+import SSA.Experimental.Bits.AutoStructs.ForLean
+
+open Set
+open Mathlib
+
+@[simp]
+lemma Mathlib.Vector.append_get_lt {x : Mathlib.Vector α n} {y : Mathlib.Vector α m} {i : Fin (n+m)} (hlt: i < n) :
+    (x.append y).get i = x.get (i.castLT hlt) := by
+  rcases x with ⟨x, hx⟩; rcases y with ⟨y, hy⟩
+  dsimp [Mathlib.Vector.append, Mathlib.Vector.get]
+  apply List.getElem_append_left
+
+@[simp]
+lemma Mathlib.Vector.append_get_ge {x : Mathlib.Vector α n} {y : Mathlib.Vector α m} {i : Fin (n+m)} (hlt: n ≤ i) :
+    (x.append y).get i = y.get ((i.cast (Nat.add_comm n m) |>.subNat n hlt)) := by
+  rcases x with ⟨x, hx⟩; rcases y with ⟨y, hy⟩
+  dsimp [Mathlib.Vector.append, Mathlib.Vector.get]
+  rcases hx
+  apply List.getElem_append_right hlt
+
+@[simp]
+def BitVec.getLsbD_cast' (bv : BitVec n) (h : n = m):
+    (h ▸ bv).getLsbD i = bv.getLsbD i := by
+  rcases h; simp
+
+
+-- this is better because card is defeq to n
+@[simps]
+instance finenum_fin : FinEnum (Fin n) where
+  card := n
+  equiv := by rfl
+
+instance (α : Type) : Inter (Language α) := ⟨Set.inter⟩
+instance (α : Type) : Union (Language α) := ⟨Set.union⟩
+
+def Mathlib.Vector.transport (v : Vector α m) (f : Fin n → Fin m) : Vector α n :=
+  Vector.ofFn fun i => v.get (f i)
+
+def BitVec.transport (f : Fin n2 → Fin n1) (bv : BitVec n1) : BitVec n2 :=
+  BitVec.ofFn fun i => bv.getLsbD (f i)
+
+@[simp]
+lemma BitVec.transport_getLsbD (f : Fin n2 → Fin n1) (bv : BitVec n1) (i : Fin n2) :
+    (bv.transport f).getLsbD i = bv.getLsbD (f i) := by
+  simp [transport]
+
+/--
+The set of `n`-tuples of bit vectors of an arbitrary width.
+-/
+structure BitVecs (n : Nat) where
+  w : Nat
+  bvs : Vector (BitVec w) n
+
+abbrev BitVecs.empty : BitVecs n := ⟨0, Mathlib.Vector.replicate n .nil⟩
+abbrev BitVecs.singleton {w : Nat} (bv : BitVec w) : BitVecs 1 := ⟨w, bv ::ᵥ .nil⟩
+abbrev BitVecs.pair {w : Nat} (bv1 bv2 : BitVec w) : BitVecs 2 := ⟨w, bv1 ::ᵥ bv2 ::ᵥ .nil⟩
+
+def BitVecs0 : Set (BitVecs n) :=
+  {⟨0, Vector.replicate n (BitVec.zero 0)⟩}
+
+-- TODO: this ought to be way easier
+@[ext (iff := false)]
+lemma BitVecs.ext (x y : BitVecs n) :
+    ∀ (heq : x.w = y.w),
+      (∀ (i : Fin n), x.bvs.get i = heq ▸ y.bvs.get i) →
+      x = y := by
+  intros heq hbvs
+  rcases x with ⟨wx, bvsx⟩
+  rcases y with ⟨wy, bvsy⟩
+  congr
+  rcases heq
+  apply heq_of_eq
+  ext i j
+  simp_all
+
+/--
+The set of `n`-tuples of bit vectors of an arbitrary width, encoded as a list of
+bit vectors of width `n`. The width of the encoded bit vectors is the length of
+the list.
+-/
+abbrev BitVecs' (n : Nat) := List (BitVec n)
+
+def enc (bvs : BitVecs n) : BitVecs' n :=
+  (List.finRange bvs.w).map (fun i =>
+    BitVec.ofFn (fun (k : Fin n) => (bvs.bvs.get k)[i]))
+
+def dec (bvs' : BitVecs' n) : BitVecs n where
+  w := bvs'.length
+  bvs := Vector.ofFn fun k => BitVec.ofFn fun i => bvs'[i].getLsbD k
+
+@[simp]
+lemma dec_nil n : dec (n := n) [] = BitVecs.empty := by
+  ext <;> simp [dec]
+
+-- The two sets are in bijection.
+
+@[simp]
+lemma enc_length (bvs : BitVecs n) : (enc bvs).length = bvs.w := by
+  simp [enc]
+
+@[simp]
+lemma dec_w (bvs' : BitVecs' n) : (dec bvs').w = bvs'.length := by
+  simp [dec]
+
+@[simp]
+lemma enc_spec (bvs : BitVecs n) (i : Fin bvs.w) (k : Fin n) :
+    (enc bvs)[i][k] = (bvs.bvs.get k)[i] := by
+  simp [enc, dec]
+
+@[simp]
+lemma dec_spec (bvs' : BitVecs' n) (k : Fin n) (i : Fin bvs'.length) :
+    ((dec bvs').bvs.get k).getLsbD i = bvs'[i].getLsbD k := by
+  simp [dec]
+
+@[simp]
+lemma dec_spec' (bvs' : BitVecs' n) (k : Fin n) (i : Fin bvs'.length) :
+    ((dec bvs').bvs.get k).getLsbD i = bvs'[i].getLsbD k := by
+  simp [dec]
+
+lemma dec_enc_w (bvs : BitVecs n) : (dec (enc bvs)).w = bvs.w := by simp [enc, dec]
+
+lemma helper_dec_enc (bvs : BitVecs n) (h : w' = bvs.w) i (j : Nat) :
+    (bvs.bvs.get i)[j]?.getD false = (h ▸ bvs.bvs.get i)[j]?.getD false := by
+  rcases h; simp
+
+@[simp]
+lemma dec_enc : Function.RightInverse (α := BitVecs' n) enc dec := by
+  intros bvs; ext1; exact dec_enc_w bvs
+  next i =>
+    simp [enc, dec]
+    ext j
+    simp
+    rw [BitVec.getLsbD_eq_getElem?_getD]
+    rw [BitVec.getElem_eq_getElem?]
+    rw [Option.get_eq_getD (fallback := false)]
+
+@[simp]
+lemma enc_dec : Function.LeftInverse (α := BitVecs' n) enc dec := by
+  intros bvs'; simp [enc, dec]
+  ext1 k
+  by_cases hin : k < (List.length bvs')
+  · simp
+    rw [List.getElem?_eq_getElem] <;> simp_all
+    ext1; simp
+  · simp; repeat rw [List.getElem?_eq_none] <;> simp_all
+
+@[simp]
+lemma dec_enc' : dec (enc bvs) = bvs := by apply dec_enc
+@[simp]
+lemma enc_dec' : enc (dec bvs') = bvs' := by apply enc_dec
+
+@[simp]
+def dec_bij {n : Nat} : Function.Bijective (dec (n := n)) := by
+  rw [Function.bijective_iff_has_inverse]; use enc; simp
+
+def dec_surj (n : Nat) : Function.Surjective (dec (n := n)) := by
+  exact Function.Bijective.surjective dec_bij
+
+def dec_inj {n : Nat} : Function.Injective (dec (n := n)) := by
+  exact Function.Bijective.injective dec_bij
+
+@[simp]
+lemma dec_snoc n (bvs' : BitVecs' n) (a : BitVec n) : dec (bvs' ++ [a]) =
+  { w := bvs'.length + 1
+    bvs := Vector.ofFn fun k => BitVec.cons (a.getLsbD k) ((dec bvs').bvs.get k) } := by
+  ext k i <;> simp [dec]
+  rw [BitVec.getLsbD_cons]
+  rcases i with ⟨i, hi⟩; simp at hi ⊢
+  split
+  next heq => simp_all
+  next h =>
+    have hlt : i < List.length bvs' := by omega
+    rw [List.getElem_append_left hlt, BitVec.ofFn_getLsbD' _ _ hlt]
+
+@[simp]
+lemma dec_enc_image : dec '' (enc '' S) = S := Function.LeftInverse.image_image dec_enc _
+
+@[simp]
+lemma env_dec_image : enc '' (dec '' S) = S :=  Function.LeftInverse.image_image enc_dec _
+
+def BitVecs.transport (f : Fin n → Fin m) (bvs : BitVecs m) : BitVecs n :=
+  { w := bvs.w, bvs := bvs.bvs.transport f }
+
+
+@[simp]
+lemma BitVecs.transport_w {bvs : BitVecs n} : (BitVecs.transport f bvs).w = bvs.w := by
+  simp [transport]
+
+@[simp]
+lemma BitVecs.transport_getElem {bvs : BitVecs m} (f : Fin n → Fin m) (i : Fin n) :
+    (bvs.transport f).bvs.get i = bvs.bvs.get (f i) := by
+  simp [transport, Mathlib.Vector.transport]
+
+def BitVecs'.transport (f : Fin n → Fin m) (bvs' : BitVecs' m): BitVecs' n :=
+  bvs'.map fun bv => bv.transport f
+
+@[simp]
+lemma BitVecs'.tranport_length {bvs' : BitVecs' n} : (BitVecs'.transport f bvs').length = bvs'.length := by
+  simp [transport]
+
+@[simp]
+lemma BitVecs'.transport_getElem {bvs' : BitVecs' m} (f : Fin n → Fin m) (i : Fin bvs'.length) :
+    (bvs'.transport f)[i] = bvs'[i].transport f := by
+  simp [transport]
+
+@[simp]
+lemma BitVecs'.transport_getElem' {bvs' : BitVecs' m} (f : Fin n → Fin m) (i : Nat) (h : i < bvs'.length) :
+    (bvs'.transport f)[i]'(by simp_all) = (bvs'[i]'h).transport f := by
+  simp [transport]
+
+-- TODO: this script generates an ill typed proof :(
+set_option debug.skipKernelTC true in
+@[simp]
+def dec_transport_idx {bvs' : BitVecs' n} (f : Fin m → Fin n) :
+    have h : (BitVecs.transport f (dec bvs')).w = (dec (BitVecs'.transport f bvs')).w := by simp
+    (dec (bvs'.transport f)).bvs.get i =  h ▸ (((dec bvs').transport f).bvs.get i) := by
+  intros h
+  simp [dec]
+  ext1 i
+  simp
+  rw [BitVecs'.transport_getElem' f i]
+  rcases i with ⟨i, hi⟩; simp
+  rw [BitVec.ofFn_getLsbD' _ i (by simp_all)]
+  simp
+
+@[simp]
+def dec_transport :
+    dec (bvs'.transport f) = (dec bvs').transport f := by
+  ext k j <;> simp
+
+@[simp]
+def enc_transport_idx {bvs : BitVecs n} (f : Fin m → Fin n) (i : Fin bvs.w) :
+    -- have h : (BitVecs.transport f (dec bvs')).w = (dec (BitVecs'.transport f bvs')).w := by simp
+    (enc (bvs.transport f))[i] = (enc bvs)[i].transport f := by
+  ext1 k; simp [enc]; rfl
+
+@[simp]
+def enc_transport :
+     enc (bvs.transport f) = (enc bvs).transport f := by
+  apply List.ext_getElem <;> simp
+  intros i hi hi'
+  have _ := enc_transport_idx f ⟨i, hi⟩
+  simp_all
+
+@[simp]
+def dec_transport_preim :
+    dec '' (BitVecs'.transport f ⁻¹' S) = BitVecs.transport f ⁻¹' (dec '' S) := by
+  ext1 bvs; simp; constructor
+  · rintro ⟨bvs', htr, hdec⟩
+    use bvs'.transport f; constructor; apply htr
+    simp [← hdec]
+  · rintro ⟨bvs', hS, hdec⟩
+    use enc bvs
+    rw [←enc_transport]
+    constructor <;> simp_all [←hdec, enc_dec]
+
+@[simp]
+def dec_transport_image (f : Fin m → Fin n) :
+    dec '' (BitVecs'.transport f '' S) = BitVecs.transport f '' (dec '' S) := by
+  ext1; simp
+
+namespace NFA
+
+def Complete' (M : NFA α σ) : Prop := ∀ q a, M.step q a ≠ ∅
+
+def Complete (M : NFA α σ) : Prop := ∀ w, Nonempty (M.eval w)
+
+lemma complete_stepSet_ne {M : NFA α σ} {hc : M.Complete'} : S ≠ ∅ → M.stepSet S a ≠ ∅ := by
+  push_neg; rintro ⟨q, hq⟩
+  have hne := hc q a
+  push_neg at hne
+  rcases hne with ⟨q', hq'⟩
+  use q'; simp [stepSet]; use q
+
+structure Deterministic (M : NFA α σ) : Prop where
+  start : M.start.Subsingleton
+  step : ∀ q a, M.step q a |>.Subsingleton
+
+attribute [simp] Deterministic.start Deterministic.step
+
+lemma deterministic_stepSet_subsingleton {M : NFA α σ} {S : Set σ} (hd : M.Deterministic) :
+    S.Subsingleton → (M.stepSet S a |>.Subsingleton) := by
+  intros hS
+  simp_all [stepSet, Set.Subsingleton]
+  intros q1' q1 hq1 hq1' q2' q2 hq2 hq2'
+  obtain rfl := hS hq1 hq2
+  obtain rfl := hd.step q1 a hq1' hq2'
+  rfl
+
+lemma deterministic_eval_subsingleton {M : NFA α σ} (hd : M.Deterministic) w :
+    M.eval w |>.Subsingleton := by
+  induction w using List.list_reverse_induction
+  case base => simp_all
+  case ind w a ih => simp; apply deterministic_stepSet_subsingleton <;> assumption
+
+private noncomputable instance {M : NFA α σ} : Decidable M.Complete :=
+  Classical.propDecidable _
+
+
+@[simp, aesop 50% unsafe]
+theorem stepSet_mono (M : NFA α σ) (S₁ S₂ : Set σ) (a : α) (h : S₁ ⊆ S₂) :
+    M.stepSet S₁ a ⊆ M.stepSet S₂ a := by
+  simp only [stepSet]; apply biUnion_mono <;> simp_all
+
+@[simp, aesop 50% unsafe]
+theorem evalFrom_mono (M : NFA α σ) (S₁ S₂ : Set σ) (x : List α) (h : S₁ ⊆ S₂) :
+    M.evalFrom S₁ x ⊆ M.evalFrom S₂ x := by
+  simp only [evalFrom]; induction' x with a x ih generalizing S₁ S₂ <;> simp_all [List.foldl_cons]
+
+def Reachable (M : NFA α σ) : Set σ := λ q ↦ ∃ w, q ∈ M.eval w
+
+def reduce (M : NFA α σ) : NFA α M.Reachable where
+  start q :=  M.start q.val
+  accept q := M.accept q.val
+  step q a q' := M.step q.val a q'.val
+
+lemma reduce_stepSet {M : NFA α σ} {q : σ} (S1 : Set M.Reachable) (S2 : Set σ) :
+    (∀ q, (∃ hq, S1 ⟨q, hq⟩) ↔ S2 q) →
+    ((∃ hq,  ⟨q, hq⟩ ∈ M.reduce.stepSet S1 a) ↔ q ∈ M.stepSet S2 a) := by
+  intros h
+  simp_all [reduce, stepSet]; constructor
+  · rintro ⟨hq, q', ⟨hr, hs1⟩, hs⟩
+    have hin : S2 q' := by rw [←h q']; use hr; apply hs1
+    use q'; constructor; apply hin; apply hs
+  · rintro ⟨q', hs2, hs⟩
+    obtain ⟨hr', hs1⟩ :=(h q').mpr hs2
+    have hr : q ∈ M.Reachable := by
+      obtain ⟨w, he⟩ := hr'
+      use (w ++ [a]); simp [stepSet]; use q'
+    use hr, q'; constructor
+    · use hr'; apply hs1
+    · apply hs
+
+lemma reduce_stepSet' {M : NFA α σ} (q : M.Reachable) (S1 : Set M.Reachable) (S2 : Set σ) :
+    (∀ q, (∃ hq, S1 ⟨q, hq⟩) ↔ S2 q) →
+    (q ∈ M.reduce.stepSet S1 a → q.val ∈ M.stepSet S2 a) := by
+  intros h; simp [←reduce_stepSet _ _ h]
+
+lemma reduce_eval {M : NFA α σ} {w} (q : σ) : (∃ hq, ⟨q, hq⟩ ∈ M.reduce.eval w) ↔ q ∈ M.eval w := by
+  induction w using List.list_reverse_induction generalizing q
+  case base => simp [reduce, Set.instMembership, Set.Mem]; intros hs; use .nil; simpa
+  case ind a w ih =>
+    simp [eval]; constructor
+    · rintro ⟨hq, hs⟩
+      apply reduce_stepSet' at hs
+      apply hs
+      apply ih
+    · rintro hs
+      rw [←reduce_stepSet] at hs
+      apply hs
+      apply ih
+
+@[simp]
+lemma reduce_spec (M : NFA α σ) : M.reduce.accepts = M.accepts := by
+  ext w; simp [accepts]; constructor
+  · rintro ⟨q, hr, ha, he⟩
+    use q
+    constructor
+    · apply ha
+    · simp_all [←reduce_eval q]
+  · rintro ⟨q, ha, he⟩
+    obtain ⟨hq, he'⟩ := reduce_eval q |>.mpr he
+    use q, hq
+    constructor
+    · apply ha
+    · simp_all [←reduce_eval q]
+
+-- TODO: M.reduce is reduced
+
+def closed_set (M : NFA α σ) (S : Set σ) := M.start ⊆ S ∧ ∀ a, M.stepSet S a ⊆ S
+
+theorem reachable_sub_closed_set (M : NFA α σ) (S : Set σ) (hcl: M.closed_set S) :
+    M.Reachable ⊆ S := by
+  rintro q ⟨w, hw⟩
+  rcases hcl with ⟨hstart, hincl⟩
+  induction w using List.list_reverse_induction generalizing q
+  case base => aesop
+  case ind w a ih =>
+    simp only [eval] at hw
+    rw [evalFrom_append_singleton, mem_stepSet] at hw
+    rcases hw with ⟨q', h1, h2⟩
+    apply ih at h1
+    suffices _ : q ∈ M.stepSet S a by aesop
+    rw [mem_stepSet]; use q'
+
+@[simps]
+def complete (M : NFA α σ) : NFA α (σ ⊕ Unit) where
+  start := { x | match x with | .inl x => x ∈ M.start | .inr () => True }
+  accept := { x | match x with | .inl x => x ∈ M.accept | .inr () => False }
+  step x a := { y |
+    match x with
+    | .inl x => match y with | .inl y => y ∈ M.step x a | .inr () => False
+    | .inr () => y = .inr () }
+
+@[simp]
+lemma accepts_cast {M : NFA α σ} (h : σ = ς): (h ▸ M).accepts = M.accepts := by
+  rcases h; simp
+
+@[simp]
+lemma step_cast {M : NFA α σ} (h : σ = ς) (q q' : σ): (h ▸ q') ∈ (h ▸ M).step (h ▸ q) a ↔ q' ∈  M.step q a := by
+  rcases h; simp
+
+@[simp]
+lemma complete_cast {M : NFA α σ} (h : σ = ς) : (h ▸ M).Complete ↔ M.Complete := by
+  rcases h; simp
+
+@[simp]
+lemma complete_stepSet {M : NFA α σ} (q : σ) :
+    (∀ q, (Sum.inl q ∈ S1) ↔ S2 q) →
+    ((.inl q ∈ M.complete.stepSet S1 a) ↔ q ∈ M.stepSet S2 a) := by
+  simp_all [complete, stepSet, Set.instMembership, Set.Mem]
+
+lemma complete_stepSet_sink {M : NFA α σ} :
+    .inr () ∈ S → .inr () ∈ M.complete.stepSet S a := by
+  simp_all [complete, stepSet, Set.instMembership, Set.Mem]
+
+@[simp]
+lemma complete_eval {M : NFA α σ} {w} (q : σ) :
+    (.inl q ∈ M.complete.eval w) ↔ q ∈ M.eval w := by
+  induction w using List.list_reverse_induction generalizing q
+  case base => simp [complete, Set.instMembership, Set.Mem]
+  case ind a w ih =>
+    simp only [eval]; constructor
+    · simp; rintro _; rw [←complete_stepSet]; assumption; apply ih
+    · simp; rintro _; rw [complete_stepSet]; assumption; apply ih
+
+@[simp]
+theorem complete_accepts (M : NFA α σ) : M.complete.accepts = M.accepts := by
+  simp [accepts]
+
+@[simp]
+theorem complete_complete (M : NFA α σ) : M.complete.Complete := by
+  intros w
+  use (.inr ())
+  induction w using List.list_reverse_induction
+  case base => simp
+  case ind w a ih =>
+    simp [eval]
+    apply complete_stepSet_sink
+    apply ih
+
+def product (accept? : Prop → Prop → Prop) (M : NFA α σ) (N : NFA α ς) : NFA α (σ × ς) where
+  step := fun (q₁, q₂) a => { (q₁', q₂') | (q₁' ∈ M.step q₁ a) ∧ (q₂' ∈ N.step q₂ a) }
+  start := { (q₁, q₂) | (q₁ ∈ M.start) ∧ (q₂ ∈ N.start) }
+  accept := { (q₁, q₂) | accept? (q₁ ∈ M.accept) (q₂ ∈ N.accept) }
+
+def inter (M : NFA α σ) (N : NFA α ς) : NFA α (σ × ς) := product And M N
+
+-- Note: the automata need to be complete!
+def union' (M : NFA α σ) (N : NFA α ς) : NFA α (σ × ς) := product Or M N
+
+def union (M : NFA α σ) (N : NFA α ς) : NFA α ((σ ⊕ Unit) × (ς ⊕ Unit)) :=
+  M.complete.union' N.complete
+
+@[simp]
+lemma product_accept {M : NFA α σ} {N : NFA α ς} :
+    (q1, q2) ∈ (M.product accept? N).accept ↔ accept? (q1 ∈ M.accept) (q2 ∈ N.accept) := by
+  simp [product]
+
+@[simp]
+lemma product_stepSet {M : NFA α σ} {N : NFA α ς} :
+    (M.product accept? N).stepSet (S1 ×ˢ S2) a = ((M.stepSet S1 a) ×ˢ (N.stepSet S2 a)) := by
+  ext ⟨q1, q2⟩; simp [product, stepSet]; constructor
+  · rintro ⟨q1', hq1, q2', hS, hq2⟩; constructor
+    · use q1'; simp_all
+    · use q2'; simp_all
+  · rintro ⟨⟨q1', h1, hs1⟩, ⟨q2', h2, hs2⟩⟩
+    use q1'; constructor; assumption; use q2'
+
+@[simp]
+lemma product_eval {M : NFA α σ} {N : NFA α ς} {w} :
+  (M.product accept? N).eval w = M.eval w ×ˢ N.eval w := by
+  unfold eval; induction w using List.list_reverse_induction
+  case base => ext; simp [product]
+  case ind w a ih => simp only [eval, evalFrom_append_singleton, product_stepSet, ih]
+
+@[simp]
+theorem inter_accepts (M : NFA α σ) (N : NFA α ς) :
+    (M.inter N).accepts = M.accepts ∩ N.accepts:= by
+  ext w; simp [accepts, inter]; constructor
+  · rintro ⟨q1, q2, ⟨_, _⟩, _, _⟩; constructor; use q1; use q2
+  · rintro ⟨⟨q1, _⟩, q2, _⟩; use q1, q2; simp_all
+
+@[simp]
+theorem union'_accepts (M : NFA α σ) (N : NFA α ς) (hcM: M.Complete) (hcN : N.Complete) :
+    (M.union' N).accepts = M.accepts ∪ N.accepts := by
+  ext w; constructor
+  · simp [accepts]
+    rintro ⟨q1, q2, ha, he⟩
+    simp [union'] at he ha
+    rcases ha with ha | ha
+    · left; use q1; simp_all
+    · right; use q2; simp_all
+  · simp [accepts]
+    rintro (⟨q1, ha, he⟩ | ⟨q2, ha, he⟩)
+    · obtain ⟨q2, he2⟩ := hcN w
+      use q1, q2; simp_all [union']
+    · obtain ⟨q1, he1⟩ := hcM w
+      use q1, q2; simp_all [union']
+
+@[simp]
+theorem union_accepts (M : NFA α σ) (N : NFA α ς) :
+    (M.union N).accepts = M.accepts ∪ N.accepts := by
+  simp [union]
+
+def flipAccept (M : NFA α σ) : NFA α σ where
+  start := M.start
+  accept := M.accept.compl
+  step := M.step
+
+@[simp]
+theorem flipAccept_eval {M : NFA α σ} : M.flipAccept.eval w = M.eval w := by
+  simp [flipAccept, eval, evalFrom]; unfold stepSet; simp
+
+@[simp]
+theorem flipAccept_accepts (M : NFA α σ) (hc : M.Complete) (hdet : M.Deterministic) :
+    M.flipAccept.accepts = M.acceptsᶜ := by
+  ext w; constructor; simp [accepts, Language.eq_def, Set.compl_def]; rintro q ha he
+  · intros q' ha' he'
+    obtain rfl := deterministic_eval_subsingleton hdet w he he'
+    simp_all [flipAccept, Set.compl]
+  · simp [accepts, Language.eq_def, Set.compl_def]
+    intros hw
+    obtain ⟨qf, hqf⟩ := hc w
+    have ha : ¬ qf ∈ M.accept := by by_contra; apply hw <;> assumption
+    use qf; simp_all [flipAccept, Set.compl]
+
+def neg (M : NFA α σ) := M.toDFA.toNFA.flipAccept
+
+@[simp]
+lemma determinize_complete (M : NFA α σ) :
+    M.toDFA.toNFA.Complete := by
+  simp [Complete, eval]
+
+@[simp]
+lemma determinize_deternistic (M : NFA α σ) :
+    M.toDFA.toNFA.Deterministic := by
+  simp [Deterministic, DFA.toNFA, toDFA]
+  constructor <;> simp
+
+@[simp]
+theorem neg_accepts (M : NFA α σ) :
+    M.neg.accepts = M.acceptsᶜ := by
+  simp [neg]
+
+
+/-
+NOTE: all that follows is defined in terms of bit vectors, even though it should
+probably be defined in terms of `Vec n α` for an arbitrary type `α`.
+-/
+
+/-- Defined as bv'[i] = bv[f i] -/
+@[simps]
+def lift (M: NFA (BitVec n1) σ) (f : Fin n1 → Fin n2) : NFA (BitVec n2) σ where
+  start := M.start
+  accept := M.accept
+  step q a := M.step q (a.transport f)
+
+@[simp]
+lemma lift_stepSet (M : NFA (BitVec n) σ) (f : Fin n → Fin m) :
+    (M.lift f).stepSet S a = M.stepSet S (a.transport f) := by
+  simp [lift, stepSet]
+
+@[simp]
+lemma lift_eval (M : NFA (BitVec n) σ) (f : Fin n → Fin m) :
+    (M.lift f).eval w = M.eval (BitVecs'.transport f w) := by
+  induction w using List.list_reverse_induction
+  case base => simp [lift, BitVecs'.transport]
+  case ind w a ih => simp [BitVecs'.transport, ih]
+
+@[simp]
+lemma lift_accepts (M : NFA (BitVec n) σ) (f : Fin n → Fin m) :
+    (M.lift f).accepts = BitVecs'.transport f ⁻¹' M.accepts := by
+  simp [accepts]
+
+@[simps]
+def proj (M: NFA (BitVec n1) σ) (f : Fin n2 → Fin n1) : NFA (BitVec n2) σ where
+  start := M.start
+  accept := M.accept
+  step q a := { q' | ∃ a', a'.transport f = a ∧ q' ∈ M.step q a' }
+
+@[simp]
+lemma proj_stepSet (M : NFA (BitVec m) σ) (f : Fin n → Fin m) :
+    (M.proj f).stepSet S a =
+      ⋃ a' ∈ BitVec.transport f ⁻¹' {a}, M.stepSet S a' := by
+  ext q; simp [proj, stepSet]; constructor
+  · rintro ⟨q', hS, a', htr, hs⟩
+    use a'; constructor; assumption; use q'
+  · rintro ⟨a', htr, q', hS, hs⟩
+    use q'; constructor; assumption; use a'
+
+@[simp]
+lemma proj_eval (M : NFA (BitVec m) σ) (f : Fin n → Fin m) :
+    (M.proj f).eval w =
+      ⋃ w' ∈ BitVecs'.transport f ⁻¹' {w}, M.eval w' := by
+  induction w using List.list_reverse_induction
+  case base => simp [proj, BitVecs'.transport]
+  case ind w a ih =>
+    ext q; simp [BitVecs'.transport]; constructor
+    · rintro ⟨a', htr, S, hrS, hqS⟩
+      rcases hrS with ⟨q', rfl⟩
+      simp [ih] at hqS
+      rcases hqS with ⟨⟨w', htr', he⟩, hs⟩
+      use w' ++ [a']; constructor
+      · simp_all; exact htr'
+      · simp; use M.step q' a'; constructor
+        on_goal 2 => assumption
+        use q'; simp_all
+    · rintro ⟨wa', heq, he⟩
+      by_cases hemp : wa' = []
+      · simp_all
+      have hdl := List.dropLast_concat_getLast hemp
+      rw [←hdl] at heq he
+      simp at heq
+      use List.getLast wa' hemp; constructor
+      · apply List.append_inj_right' at heq; simp_all
+      · obtain rfl := List.append_inj_left' heq (by simp)
+        simp at he; rcases he with ⟨S, ⟨q', rfl⟩, hqS⟩
+        simp at hqS; rcases hqS with ⟨he, hs⟩
+        simp only [stepSet, mem_iUnion, exists_prop]
+        use q'
+        simp [ih]; constructor
+        on_goal 2 => assumption
+        use wa'.dropLast
+        simp_all [BitVecs'.transport]
+
+@[simp]
+lemma proj_accepts (M : NFA (BitVec m) σ) (f : Fin n → Fin m) :
+    (M.proj f).accepts = BitVecs'.transport f '' M.accepts := by
+  ext w; simp [accepts]; constructor
+  · rintro ⟨q, ha, w', htr, he⟩
+    use w'; simp [htr]; use q
+  · rintro ⟨w', ⟨q, he, hv⟩, htr⟩
+    use q; simp [he]; use w'
