SSA/Experimental/Bits/AutoStructs/GoodNFA.lean
@@ -1,0 +1,94 @@
+import Batteries.Data.Fin.Basic
+import Mathlib.Computability.NFA
+import Mathlib.Data.FinEnum
+import Mathlib.Data.Vector.Basic
+import Mathlib.Data.Vector.Defs
+import SSA.Experimental.Bits.AutoStructs.ForLean
+import SSA.Experimental.Bits.AutoStructs.ForMathlib
+
+structure GoodNFA (n : Nat) where
+  σ : Type
+  M : NFA (BitVec n) σ
+  -- all reachable? complete? etc
+
+namespace GoodNFA
+
+/--
+The encoded tuples of bit vectors accepted by an automaton.
+-/
+def accepts' (M : GoodNFA n) : Set (BitVecs' n) := M.M.accepts
+
+/--
+The tuples of bit vectors accepted by an automaton.
+-/
+def accepts (M : GoodNFA n) : Set (BitVecs n) := dec '' M.accepts'
+
+
+noncomputable def complete (M : GoodNFA n) : GoodNFA n where
+  σ := _
+  M := M.M.complete
+
+
+def product (final? : Prop → Prop → Prop) (M N : GoodNFA n) : GoodNFA n where
+  σ := _
+  M := M.M.product final? N.M
+
+def inter (M N : GoodNFA n) : GoodNFA n := ⟨_, M.M.inter N.M⟩
+
+lemma inter_eq (M N : GoodNFA n) : M.inter N = GoodNFA.product And M N := by
+  simp [inter, product, NFA.inter]
+
+@[simp]
+lemma inter_accepts (M N : GoodNFA n) :
+    (M.inter N).accepts = M.accepts ∩ N.accepts := by
+  simp [accepts, accepts', inter, Set.image_inter dec_inj]
+
+def union (M N : GoodNFA n) : GoodNFA n := ⟨_, M.M.union N.M⟩
+
+lemma union_eq (M N : GoodNFA n) : M.union N = GoodNFA.product Or M.complete N.complete := by
+  simp [union, product, NFA.union, NFA.union', complete]
+
+@[simp]
+lemma union_accepts (M N : GoodNFA n) :
+    (M.union N).accepts = M.accepts ∪ N.accepts := by
+  simp [accepts, accepts', union]; rw [Set.image_union]
+
+def neg (M : GoodNFA n) : GoodNFA n where
+  σ := _
+  M := M.M.neg
+
+@[simp]
+lemma neg_accepts (M : GoodNFA n) :
+    M.neg.accepts = M.acceptsᶜ:= by
+  simp [accepts, accepts', neg, Set.image_compl_eq (dec_bij)]
+
+def reduce (M : GoodNFA n) : GoodNFA n where
+  σ := _
+  M := M.M.reduce
+
+@[simp]
+lemma reduce_accepts {M : GoodNFA n} : M.reduce.accepts = M.accepts := by
+  simp [reduce, accepts, accepts']
+
+
+def determinize (M : GoodNFA n) : GoodNFA n where
+  σ := _
+  M := M.M.toDFA.toNFA
+
+def lift (f : Fin n → Fin m) (M : GoodNFA n) : GoodNFA m where
+  σ := _
+  M := M.M.lift f
+
+def proj (f : Fin m → Fin n) (M : GoodNFA n) : GoodNFA m where
+  σ := _
+  M := M.M.proj f
+
+@[simp]
+lemma lift_accepts (M : GoodNFA n) (f : Fin n → Fin m) :
+    (M.lift f).accepts = BitVecs.transport f ⁻¹' M.accepts := by
+  simp [accepts, accepts', lift]
+
+@[simp]
+lemma proj_accepts (M : GoodNFA m) (f : Fin n → Fin m) :
+    (M.proj f).accepts = BitVecs.transport f '' M.accepts := by
+  simp [accepts, accepts', proj]
